

Daily Integral

Hard Derivatives

Author: Yusaf Sultan

Contents

1. 05/02/2026: $f(x) = \frac{\arctan^5(x)}{\sqrt{\arccos^4(x)}} + \frac{\sin^2(x)}{\cot^2(x)}$, $f'(0.7) = ?$	3
2. 06/02/2026: $\sqrt[5]{\ln(3 + \cos(e^{x^2}))} \tan(\arctan(x^3) + \sqrt{x+2})$, $f'(0) = ?$	5
3. 17/02/2026: $f(x) = x^{x^{x^{\dots}}}$, $f'(\frac{6}{5}) = ?$	7
4. 24/02/2026: $f(x) = \sin(x)^{\cos(x)^{\tan(x)}}$, $f'(\frac{\pi}{4}) = ?$	8

1. 05/02/2026: $f(x) = \frac{\arctan^5(x)}{\sqrt{\arccos^4(x)}} + \frac{\sin^2(x)}{\cot^2(x)}$, $f'(0.7) = ?$

To start with the derivative is defined and split into two separate derivatives using the **sum rule**, this is shown in **Eq. 1**.

$$f'(x) = \frac{d}{dx}(f(x)) = \frac{d}{dx} \left(\frac{\arctan^5(x)}{\sqrt{\arccos^4(x)}} \right) + \frac{d}{dx} \left(\frac{\sin^2(x)}{\cot^2(x)} \right) \quad (1)$$

The first section of the derivative can then be solved using a combination of the **quotient rule** and **chain rule**, the u and v s are shown in **Eq. 2**.

$$\text{Let } u = \arctan^5(x) \quad v = \sqrt{\arccos^4(x)} \quad (2)$$

To differentiate u and v , chain rule can be used. To obtain $\frac{du}{dx}$ the chain rule is applied in **Eq. 3**.

$$u = \arctan^5(x) \longrightarrow \text{Let } z = \arctan(x) \therefore u = z^5 \quad (3.1)$$

$$\frac{dz}{dx} = \frac{1}{1+x^2} \quad \frac{du}{dz} = 5z^4 \quad (3.2)$$

$$\frac{du}{dx} = \frac{du}{dz} \cdot \frac{dz}{dx} = \frac{5z^4}{1+x^2} = \frac{5\arctan^4(x)}{1+x^2} \quad (3.3)$$

To obtain an expression for $\frac{dv}{dx}$ chain rule can be used twice, this is shown in **Eq. 4**.

$$v = \sqrt{\arccos^4(x)} \longrightarrow \text{Let } z = \arccos^4(x) \therefore v = \sqrt{z} \quad (4.1)$$

$$z = \arccos^4(x) \longrightarrow \text{Let } q = \arccos(x) \therefore z = q^4 \quad (4.2)$$

$$\frac{dz}{dq} = 4q^3 \quad \frac{dq}{dx} = \frac{1}{\sqrt{1-x^2}} \quad \frac{dv}{dz} = \frac{1}{2\sqrt{z}} \quad (4.3)$$

$$\frac{dv}{dx} = \frac{dv}{dz} \cdot \frac{dz}{dx} = \frac{dv}{dz} \cdot \frac{dz}{dq} \cdot \frac{dq}{dx} = \frac{4q^3}{2\sqrt{z}(\sqrt{1-x^2})} = \frac{4\arccos^3(x)}{2\sqrt{\arccos^4(x)}(\sqrt{1-x^2})} = \dots \quad (4.4)$$

$$\dots = \frac{2\arccos(x)}{\sqrt{1-x^2}} \quad (4.5)$$

Now that the expressions for $\frac{du}{dx}$ and $\frac{dv}{dx}$ have been obtained, the quotient rule can be applied to obtain $f'(x)$ for the first term, this is shown in **Eq. 5**.

$$\text{Let } u = \arctan^5(x) \quad v = \sqrt{\arccos^4(x)} \quad (5.1)$$

$$\frac{du}{dx} = \frac{5\arctan^4(x)}{1+x^2} \quad \frac{dv}{dx} = \frac{2\arccos(x)}{\sqrt{1-x^2}} \quad (5.2)$$

$$A' = \frac{1}{v^2} \left[\frac{du}{dx} v - u \frac{dv}{dx} \right] = \frac{1}{\arccos^4(x)} \left[\frac{5\arctan^4(x)\arccos^2(x)}{1+x^2} + \frac{2\arctan^5(x)\arccos(x)}{\sqrt{1-x^2}} \right] \quad (5.3)$$

The second section of the expression can first be simplified using trigonometric expressions and then the quotient rule can be applied. The initial trig simplification is shown in **Eq. 6**.

$$B = \frac{\sin^2(x)}{\cot^2(x)} = \frac{\sin^4(x)}{\cos^2(x)} \quad \text{As } \cot x = \frac{\cos x}{\sin x} \quad (6)$$

Eq. 6 can be differentiated using a mixture of chain rule and quotient rule, the u and v are defined in **Eq. 7**

$$\text{Let } u = \sin^4(x) \quad v = \cos^2(x) \quad (7)$$

An expression for $\frac{du}{dx}$ can be generated by using the chain rule shown in **Eq. 8**.

$$u = \sin^4(x) \longrightarrow \text{Let } z = \sin(x) \therefore u = z^4 \quad (8.1)$$

$$\frac{dz}{dx} = \cos(x) \quad \frac{du}{dz} = 4z^3 \quad (8.2)$$

$$\frac{du}{dx} = \frac{du}{dz} \cdot \frac{dz}{dx} = 4 \cos(x) z^3 = 4 \cos(x) \sin^3(x) \quad (8.3)$$

An expression for $\frac{dv}{dx}$ can be generated by using the chain rule shown in **Eq. 9**.

$$u = \cos^2(x) \longrightarrow \text{Let } z = \cos(x) \therefore u = z^2 \quad (9.1)$$

$$\frac{dz}{dx} = -\sin(x) \quad \frac{du}{dz} = 2z \quad (9.2)$$

$$\frac{du}{dx} = \frac{du}{dz} \cdot \frac{dz}{dx} = -2 \sin(x) z = -2 \sin(x) \cos(x) \quad (9.3)$$

Now that an expression for $\frac{du}{dx}$ and $\frac{dv}{dx}$ have been defined, the quotient rule can be applied, as shown in **Eq. 10**

$$\text{Let } u = \sin^4(x) \quad v = \cos^2(x) \quad (10.1)$$

$$\frac{du}{dx} = 4 \sin^3(x) \cos(x) \quad \frac{dv}{dx} = -2 \sin(x) \cos(x) \quad (10.2)$$

$$B' = \frac{1}{v^2} \left[\frac{du}{dx} v - u \frac{dv}{dx} \right] = \frac{1}{\cos^2(x)} [4 \sin^3(x) \cos^3(x) + 2 \sin^5(x) \cos(x)] = \dots \quad (10.3)$$

$$\dots = 4 \sin^3(x) \cos(x) + \frac{2 \sin^5(x)}{\cos(x)} \quad (10.4)$$

Combining the A' and B' terms together yield a final expression for $f'(x)$ can be constructed, this is shown in **Eq. 10**.

$$f'(x) = \frac{1}{\arccos^4(x)} \left[\frac{5 \arctan^4(x) \arccos^2(x)}{1+x^2} + \frac{2 \arctan^5(x) \arccos(x)}{\sqrt{1-x^2}} \right] + \dots \quad (11.1)$$

$$\dots + 4 \sin^3(x) \cos(x) + \frac{2 \sin^5(x)}{\cos(x)} \quad (11.2)$$

To solve the question, $x = 0$ is substituted into $f'(0)$, which is shown in **Eq. 11**.

$$f'(0) = 2.498(0.300 + 0.189) + 0.818 + 0.2901 \approx 2.32 \quad (2 \text{ d.p}) \quad (12)$$

2. 06/02/2026: $\sqrt[5]{\ln(3 + \cos(e^{x^2}))} \tan(\arctan(x^3) + \sqrt{x+2}), f'(0) = ?$

To solve this derivative a combination of **product rule** and **chain rule** can be used, the u and v s are shown in **Eq. 13**.

$$\text{Let } u = \sqrt[5]{\ln(3 + \cos(e^{x^2}))} \quad v = \tan(\arctan(x^3) + \sqrt{x+2}) \quad (13)$$

To obtain an expression for $\frac{du}{dx}$ chain rule can be repeatedly used, this is shown in **Eq. 14**.

$$u = \sqrt[5]{\ln(3 + \cos(e^{x^2}))} \rightarrow \text{Let } A = \ln(3 + \cos(e^{x^2})) \therefore u = \sqrt[5]{A} \quad (14.1)$$

$$A = \ln(3 + \cos(e^{x^2})) \rightarrow \text{Let } B = 3 + \cos(e^{x^2}) \therefore A = \ln(B) \quad (14.2)$$

$$B = 3 + \cos(e^{x^2}) \rightarrow \text{Let } C = e^{x^2} \therefore B = 3 + \cos(C) \quad (14.3)$$

$$C = e^{x^2} \rightarrow \text{Let } D = x^2 \therefore C = e^D \quad (14.4)$$

$$\frac{du}{dA} = \frac{1}{5(\sqrt[5]{A})^4} \quad \frac{dA}{dB} = \frac{1}{B} \quad \frac{dB}{dC} = -\sin(C) \quad \frac{dC}{dD} = e^D \quad \frac{dD}{dx} = 2x \quad (14.5)$$

$$\frac{du}{dx} = \frac{dA}{dB} \cdot \frac{dB}{dC} \cdot \frac{dC}{dD} \cdot \frac{dD}{dx} \cdot \frac{du}{dA} = \dots \quad (14.6)$$

$$\dots = \frac{1}{B} \cdot -\sin(C) \cdot e^D \cdot 2x \cdot \frac{1}{5(\sqrt[5]{A})^4} = \frac{-2xe^{x^2} \sin(e^{x^2})}{5(\sqrt[5]{\ln(3 + \cos(e^{x^2}))})^4 (3 + \cos(e^{x^2}))} \quad (14.7)$$

The v term can be differentiated using chain rule, however each term within the tan brackets will need to have chain rule applied separately, this is done for the $\arctan(x^3)$ term in **Eq. 15**.

$$A_1 = \arctan(x^3) \text{ Let } z = x^3 \therefore A_1 = \arctan(z) \quad (15.1)$$

$$\frac{dz}{dx} = 3x^2 \quad \frac{dA_1}{dz} = \frac{1}{1+z^2} \quad (15.2)$$

$$\frac{dA_1}{dx} = \frac{dA_1}{dz} \cdot \frac{dz}{dx} = \frac{3x^2}{1+x^6} \quad (15.3)$$

A similar process can be done for the second term ($\sqrt{x+2}$) which is shown in **Eq. 16**.

$$A_2 = \sqrt{x+2} \text{ Let } z = x+2 \therefore A_2 = \sqrt{z} \quad (16.1)$$

$$\frac{dz}{dx} = 1 \quad \frac{dA_2}{dz} = \frac{1}{2\sqrt{z}} \quad (16.2)$$

$$\frac{dA_2}{dx} = \frac{dA_2}{dz} \cdot \frac{dz}{dx} = \frac{1}{\sqrt{x+2}} \quad (16.3)$$

Now that expressions for $\frac{dA_1}{dx}$ and $\frac{dA_2}{dx}$ have been obtained chain rule can be constructed into an expression for $\frac{dv}{dx}$, shown in **Eq. 17**.

$$v = \tan(\arctan(x^3) + \sqrt{x+2}) \text{ Let } z = \arctan(x^3) + \sqrt{x+2} \therefore v = \tan(z) \quad (17.1)$$

$$\frac{dz}{dx} = \frac{dA_1}{dx} + \frac{dA_2}{dx} = \frac{3x^2}{1+x^6} + \frac{1}{\sqrt{x+2}} \quad \frac{dv}{dz} = \sec^2(z) \quad (17.2)$$

$$\frac{dv}{dx} = \frac{dv}{dz} \cdot \frac{dz}{dx} = \sec^2(z) \left[\frac{3x^2}{1+x^6} + \frac{1}{\sqrt{x+2}} \right] = \dots \quad (17.3)$$

$$\dots = \frac{3x^2 \sec^2(\arctan(x^3) + \sqrt{x+2})}{1+x^6} + \frac{\sec^2(\arctan(x^3) + \sqrt{x+2})}{\sqrt{x+2}} \quad (17.4)$$

3. 17/02/2026: $f(x) = x^{x^{x^{\cdots}}}$, $f'(\frac{6}{5}) = ?$

To solve this question, **implicit differentiation** can be used in combination with an **iterative processes**. Initially the function can be simplified into an expression that can be differentiated, shown in **Eq. 18**.

$$y = x^{x^{x^{\cdots}}} \longrightarrow y = x^y \longrightarrow \ln(y) = y \ln(x) \quad (18)$$

Each term in **Eq. 18** can be differentiated, using product rule for the $x \ln(y)$ term, shown in **Eq. 19**.

$$A' = \frac{d}{dx}(\ln(y)) = \frac{1}{y} \frac{dy}{dx} \quad (19.1)$$

$$\text{Let } u = y \quad v = \ln(x) \quad (19.2)$$

$$\frac{du}{dx} = \frac{dy}{dx} \quad \frac{dv}{dx} = \frac{1}{x} \quad (19.3)$$

$$B' = u \frac{dv}{dx} + \frac{du}{dx} v = \frac{y}{x} + \frac{dy}{dx} \ln(x) \quad (19.4)$$

$$\therefore \frac{1}{y} \frac{dy}{dx} = \frac{y}{x} + \frac{dy}{dx} \ln(x) \longrightarrow \frac{dy}{dx} = \frac{y^2}{x - xy \ln(x)} \quad (19.5)$$

An approximate value of y can be found by using the simplified form of the expression and iterating with an initial guess to find the true value of y when $x = \frac{6}{5}$, this is shown in **Eq. 20**.

$$y_{n+1} = x^{y_n} \quad \text{Let } x = \frac{6}{5} = 1.2, \quad y_0 = 2 \quad (20.1)$$

$$y_1 = x^{y_0} = 1.2^2 = 1.44 \quad (20.2)$$

$$y_2 = x^{y_1} = 1.2^{1.44} = 1.30 \quad (20.3)$$

$$\dots \quad (20.4)$$

$$y_7 = 1.2577 \therefore y \approx 1.26 \quad (20.5)$$

The values of x and y can then be inputted into $f'(x)$ to obtain a solution for the problem, shown in **Eq. 21**.

$$f'(x) = \frac{y^2}{x - xy \ln(x)} = \frac{1.26^2}{1.2 - 1.2 \times 1.26 \times \ln(1.2)} \approx 1.71 \quad (2 \text{ d.p.}) \quad (21)$$

4. 24/02/2026: $f(x) = \sin(x)^{\cos(x)\tan(x)}$, $f'(\frac{\pi}{4}) = ?$

This derivative can be solved by first taking natural logarithms twice to simplify the expression, this process is shown in **Eq. 22**.

$$y = \sin(x)^{\cos(x)\tan(x)} \longrightarrow \ln(\ln(y)) = \tan(x) \ln(\cos(x)) + \ln(\ln(\sin(x))) \quad (22)$$

Eq. 22 can be differentiated implicitly with each term differentiated by using a mixture of chain rule and product rule. This is shown for $\ln(\ln(y))$ in **Eq. 23**.

$$\frac{d}{dx}[\ln(\ln(y))] \longrightarrow A = \ln(\ln(y)) \text{ Let } z = \ln(y) \therefore A = \ln(z) \quad (23.1)$$

$$z = \ln(y) \text{ Let } q = y \therefore z = \ln(q) \quad (23.2)$$

$$\frac{dq}{dx} = \frac{dy}{dx} \quad \frac{dz}{dq} = \frac{1}{q} \quad \frac{dA}{dz} = \frac{1}{z} \quad (23.3)$$

$$\frac{dA}{dx} = \frac{dA}{dz} \cdot \frac{dz}{dx} = \frac{dA}{dz} \cdot \frac{dz}{dq} \cdot \frac{dq}{dx} = \frac{dy}{dx} \frac{1}{zq} = \frac{dy}{dx} \frac{1}{y \ln(y)} \quad (23.4)$$

The $\tan(x) \ln(\cos(x))$ can be differentiated using product rule and chain rule to differentiate $\ln(\cos(x))$, this is shown in **Eq. 24**.

$$\frac{d}{dx}[\tan(x) \ln(\cos(x))] \longrightarrow \text{Let } u = \tan(x) \quad v = \ln(\cos(x)) \quad (24.1)$$

$$(24.2)$$

$$\text{Let } z = \cos(x) \therefore v = \ln(z) \quad (24.3)$$

$$\frac{dz}{dx} = -\sin(x) \quad \frac{dv}{dz} = \frac{1}{z} \quad (24.4)$$

$$\frac{dv}{dx} = \frac{dv}{dz} \cdot \frac{dz}{dx} = -\frac{\sin(x)}{z} = -\tan(x) \quad (24.5)$$

$$(24.6)$$

$$\therefore u = \tan(x) \quad v = \ln(\cos(x)) \quad (24.7)$$

$$\frac{du}{dx} = \sec^2(x) \quad \frac{dv}{dx} = -\tan(x) \quad (24.8)$$

$$\frac{dB}{dx} = u \frac{dv}{dx} + \frac{du}{dx} v = \sec^2 \ln(\cos(x)) - \tan^2(x) \quad (24.9)$$

The $\ln(\ln(\sin(x)))$ term can be differentiated by using chain rule twice, this is shown in **Eq. 25**.

$$\frac{d}{dx}[\ln(\ln(\sin(x)))] \longrightarrow C = \ln(\ln(\sin(x))) \text{ Let } z = \ln(\sin(x)) \therefore C = \ln(z) \quad (25.1)$$

$$z = \ln(\sin(x)) \text{ Let } q = \sin(x) \therefore z = \ln(q) \quad (25.2)$$

$$\frac{dq}{dx} = \cos(x) \quad \frac{dz}{dq} = \frac{1}{q} \quad \frac{dC}{dz} = \frac{1}{z} \quad (25.3)$$

$$\frac{dC}{dx} = \frac{dC}{dz} \cdot \frac{dz}{dx} = \frac{dC}{dz} \cdot \frac{dz}{dq} \cdot \frac{dq}{dx} = \frac{\cos(x)}{zq} = \frac{\cos(x)}{\sin(x) \ln(\sin(x))} = \frac{\cot(x)}{\ln(\sin(x))} \quad (25.4)$$

Each of these terms can be combined to form one expression, this is shown in **Eq. 26** rearranged for $\frac{dy}{dx}$.

$$A' = B' + C' \longrightarrow \frac{dy}{dx} \frac{1}{y \ln(y)} = \sec^2 \ln(\cos(x)) - \tan^2(x) + \frac{\cot(x)}{\ln(\sin(x))} = \dots \quad (26.1)$$

$$\dots = \frac{dy}{dx} = y \ln(y) \left[\sec^2 \ln(\cos(x)) + \frac{\cot(x)}{\ln(\sin(x))} - \tan^2(x) \right] \quad (26.2)$$

The value of y can be determined using the original expression, substituting $x = \frac{\pi}{4}$. These values are inputted into **Eq. 26** to obtain a solution, this is shown in **Eq. 27**.

$$y(x) = \sin(x)^{\cos(x) \tan(x)} \longrightarrow y\left(\frac{\pi}{4}\right) = \sin\left(\frac{\pi}{4}\right)^{\cos\left(\frac{\pi}{4}\right) \tan\left(\frac{\pi}{4}\right)} \approx 0.782654 \quad (27.1)$$

$$\frac{dy}{dx} \Big|_{x=\frac{\pi}{4}} \approx 0.88 \quad (2 \text{ d.p}) \quad (27.2)$$